

LA-HW1

Zahra Rafati

November 28, 2024

Question 1

- (a) $\mathbf{z} + \mathbf{u} \stackrel{1}{=} \mathbf{u} + \mathbf{z} \stackrel{3}{=} \mathbf{u}$.
- (b) Consider there exists a \mathbf{w} such that $\mathbf{u} + \mathbf{w} = \mathbf{u}$ for every $\mathbf{u} \in \mathbf{V}$.
 $\mathbf{u} + \mathbf{w} = \mathbf{u} \xrightarrow{\mathbf{u}=\mathbf{z}} \mathbf{z} + \mathbf{w} = \mathbf{z} \stackrel{1}{=} \mathbf{w} + \mathbf{z} \stackrel{3}{=} \mathbf{w}$.
Therefore, $\mathbf{z} = \mathbf{w}$.
- (c) $\mathbf{z}' = \mathbf{w} \xrightarrow{+\mathbf{z}} \mathbf{z} + \mathbf{z}' = \mathbf{z} + \mathbf{w}$.
 $\mathbf{z} + \mathbf{z}' \stackrel{4}{=} \mathbf{z}$.
 $\mathbf{z} + \mathbf{w} \stackrel{a}{=} \mathbf{w}$.
Thus, $\mathbf{z} = \mathbf{w}$.
- (d) $\mathbf{u} + \mathbf{w} = \mathbf{z} \stackrel{4}{=} \mathbf{u} + \mathbf{u}' \xrightarrow{+\mathbf{u}^{-1}} \mathbf{u}' + \mathbf{u} + \mathbf{w} = \mathbf{u}' + \mathbf{u} + \mathbf{u}'$.
Using (4, 1), $\mathbf{z} + \mathbf{w} = \mathbf{z} + \mathbf{u}' \xrightarrow{a} \mathbf{z} = \mathbf{u}'$.
- (e) $\mathbf{u} + 0\mathbf{u} \stackrel{5}{=} 1\mathbf{u} + 0\mathbf{u} \stackrel{8}{=} (1+0)\mathbf{u} = 1\mathbf{u} \stackrel{5}{=} \mathbf{u} \xrightarrow{3b} 0\mathbf{u} = \mathbf{z}$.
- (f) $a\mathbf{z} \stackrel{e}{=} a(0\mathbf{u}) \stackrel{6}{=} (a0)\mathbf{u} = 0\mathbf{u} \stackrel{e}{=} \mathbf{z}$.
- (g) $0\mathbf{u} = (1-1)\mathbf{u} = 1\mathbf{u} + (-1)\mathbf{u} = \mathbf{u} + (-1)\mathbf{u}$.
 $\mathbf{z} = \mathbf{u} + \mathbf{u}^{-1}$.
 $0\mathbf{u} = \mathbf{z} \rightarrow \mathbf{u} + \mathbf{u}^{-1} = \mathbf{u} + (-1)\mathbf{u} \xrightarrow{d} \mathbf{u}^{-1} = (-1)\mathbf{u}$.

Question 2

Let

$$\mathbf{Ax} = \mathbf{z}, \quad \text{where } \mathbf{A} = \begin{bmatrix} a_1 & a_2 & \cdots & a_n \end{bmatrix}, \quad \mathbf{x} = \begin{bmatrix} x_1 \\ \vdots \\ x_n \end{bmatrix}.$$

$$\mathbf{Ax} = x_1\mathbf{a}_1 + x_2\mathbf{a}_2 + \cdots + x_n\mathbf{a}_n.$$

If $\mathbf{a}_k = \mathbf{a}_k + 0$, then

$$\mathbf{a}_k = \mathbf{a}_k + x_1 \mathbf{a}_1 + \cdots + x_n \mathbf{a}_n \implies x_1 \mathbf{a}_1 + \cdots + (x_k + 1) \mathbf{a}_k + \cdots + x_n \mathbf{a}_n = \mathbf{A} \mathbf{x}'.$$

The problem states that for every \mathbf{x} , the equation $\mathbf{A} \mathbf{x} = 0$ holds. Therefore, we constructed a new \mathbf{x} :

$$\mathbf{A} \mathbf{x}' = 0 \implies \mathbf{a}_k = 0 \implies \mathbf{A} = \mathbf{0}_{m \times n}.$$

Question 3

Let

$$\mathbf{x} = m_1 \mathbf{x}_1 + \cdots + m_n \mathbf{x}_n.$$

Then,

$$\mathbf{A} \mathbf{x} = m_1 \mathbf{A} \mathbf{x}_1 + \cdots + m_n \mathbf{A} \mathbf{x}_n \implies \mathbf{A} \mathbf{x} = 0.$$

In Question 2, we proved that since \mathbf{x} can be any vector, if $\mathbf{A} \mathbf{x} = 0$, then $\mathbf{A} = 0$. Therefore:

$$\mathbf{A} = \mathbf{0}_{m \times n}.$$

Question 4

$$\mathbf{A} \mathbf{x} = \mathbf{x} \implies \mathbf{A} \mathbf{x} - \mathbf{x} = 0 \implies (\mathbf{A} - \mathbf{I}) \mathbf{x} = 0.$$

$$\mathbf{A} \mathbf{x} - \mathbf{I}_n \mathbf{x} = 0 \implies (\mathbf{A} - \mathbf{I}_n) \mathbf{x} = 0.$$

Based on Question 2, if the above equation holds for every \mathbf{x} , then $\mathbf{A} - \mathbf{I}_n = 0$.

$$\mathbf{A} = \mathbf{I}_n.$$

Question 5

Let

$$\mathbf{A} = \begin{bmatrix} 1 & 0 & \cdots & 0 \\ 0 & 0 & \cdots & 0 \\ \vdots & \vdots & \ddots & \vdots \\ 0 & 0 & \cdots & 0 \end{bmatrix}, \quad \mathbf{x} = \begin{bmatrix} 1 \\ 0 \\ \vdots \\ 0 \end{bmatrix}.$$

Then,

$$\mathbf{A} \mathbf{x} = \begin{bmatrix} 1 \\ 0 \\ \vdots \\ 0 \end{bmatrix} = \mathbf{x}.$$

Question 6

Given:

$$x_1 \mathbf{a}_1 + \cdots + x_n \mathbf{a}_n = \mathbf{0} \implies \mathbf{x} = \begin{bmatrix} x_1 \\ x_2 \\ \vdots \\ x_n \end{bmatrix} = \mathbf{0}.$$

Substituting:

$$x_1 \mathbf{a}'_1 + \cdots + x_n \mathbf{a}_n = \mathbf{0} \implies x_1(\mathbf{a}_1 + \beta \mathbf{a}_2) + \cdots + x_n \mathbf{a}_n = \mathbf{0}.$$

$$\implies x_1 \mathbf{a}_1 + (x_2 + \beta x_1) \mathbf{a}_2 + \cdots + x_n \mathbf{a}_n = \mathbf{0}.$$

Since:

$$x_1 = 0 \implies \beta x_1 = 0.$$

And:

$$x_2 = 0.$$

Thus:

$$x_2 + \beta x_1 = 0.$$

Question 7

(a)

$$\langle \mathbf{A}, \mathbf{B} \rangle = \sum_{i=1}^m \sum_{j=1}^n \mathbf{A}_{ij} \mathbf{B}_{ij}.$$

$$\text{trace}(\mathbf{S}) = \sum_i \mathbf{S}_{ii}.$$

Let $\mathbf{A} \in \mathbb{R}^{m \times n}$ and $\mathbf{B} \in \mathbb{R}^{n \times t}$, then:

$$\mathbf{C}_{m \times t} = \mathbf{A}_{m \times n} \mathbf{B}_{n \times t}, \quad c_{ij} = \sum_{k=1}^n \mathbf{a}_{ik} \mathbf{b}_{kj}.$$

$$(I) \quad (\mathbf{A}^T \mathbf{B})_{ij} = \sum_{k=1}^m \mathbf{a}_{ki} \mathbf{b}_{kj} \implies \text{trace}(\mathbf{A}^T \mathbf{B}) =$$

$$\sum_{i=1}^n \sum_{k=1}^m \mathbf{a}_{ki} \mathbf{b}_{ki} = \sum_{k=1}^m \sum_{i=1}^n \mathbf{a}_{ki} \mathbf{b}_{ki} = \langle \mathbf{A}, \mathbf{B} \rangle.$$

$$(II) \quad (\mathbf{B}^T \mathbf{A})_{ij} = \sum_{k=1}^m \mathbf{b}_{ki} \mathbf{a}_{kj} \implies \text{trace}(\mathbf{B}^T \mathbf{A}) =$$

$$\sum_{i=1}^n \sum_{k=1}^m \mathbf{b}_{ki} \mathbf{a}_{ki} = \sum_{k=1}^m \sum_{i=1}^n \mathbf{a}_{ki} \mathbf{b}_{ki} = \langle \mathbf{A}, \mathbf{B} \rangle.$$

$$(III) \quad (\mathbf{AB}^T)_{ij} = \sum_{k=1}^n \mathbf{a}_{ik} \mathbf{b}_{jk} \implies \text{trace}(\mathbf{AB}^T) =$$

$$\sum_{i=1}^m \sum_{k=1}^n \mathbf{a}_{ik} \mathbf{b}_{ik} = \langle \mathbf{A}, \mathbf{B} \rangle.$$

(b)

$$(IV) \quad \langle \mathbf{AB}, \mathbf{C} \rangle \stackrel{(I)}{=} \text{trace}((\mathbf{AB})^T \mathbf{C}) = \text{trace}(\mathbf{B}^T \mathbf{A}^T \mathbf{C})$$

$$= \text{trace}(\mathbf{B}^T (\mathbf{A}^T \mathbf{C})) \stackrel{(I)}{=} \langle \mathbf{B}, \mathbf{A}^T \mathbf{C} \rangle.$$

$$(V) \quad \langle \mathbf{AB}, \mathbf{C} \rangle \stackrel{(III)}{=} \text{trace}(\mathbf{ABC}^T) = \text{trace}(\mathbf{A}(\mathbf{CB}^T)^T)$$

$$= \langle \mathbf{A}, \mathbf{CB}^T \rangle.$$

Question 8

Let

$$\mathbf{A} = \begin{bmatrix} a_{11} & a_{12} & \cdots & a_{1n} \\ 0 & a_{22} & \cdots & a_{2n} \\ \vdots & \vdots & \ddots & \vdots \\ 0 & 0 & \cdots & a_{nn} \end{bmatrix},$$

where \mathbf{A} is an upper triangular matrix. We assume $a_{kk} = 0$ for $1 \leq k \leq n$. Our goal is to prove that there exists a non-zero vector \mathbf{x} such that $\mathbf{Ax} = 0$.

Define:

$$\mathbf{A} = \begin{bmatrix} \mathbf{A}_1 & \mathbf{A}_2 \\ 0 & \mathbf{A}_3 \end{bmatrix}.$$

Where $\mathbf{A}_{311} = 0$.

$$\mathbf{Ax} = 0 \implies \begin{bmatrix} \mathbf{A}_1 & \mathbf{A}_2 \\ 0 & \mathbf{A}_3 \end{bmatrix} \mathbf{x} = 0 \implies \mathbf{x} = \begin{bmatrix} -\mathbf{A}_1^{-1} \mathbf{A}_2 \mathbf{z} \\ \mathbf{z} \end{bmatrix}.$$

$$\mathbf{Ax} = \begin{bmatrix} \mathbf{A}_1 & \mathbf{A}_2 \\ 0 & \mathbf{A}_3 \end{bmatrix} \begin{bmatrix} -\mathbf{A}_1^{-1} \mathbf{A}_2 \mathbf{z} \\ \mathbf{z} \end{bmatrix} = \begin{bmatrix} -\mathbf{A}_1 \mathbf{A}_1^{-1} \mathbf{A}_2 \mathbf{z} + \mathbf{A}_2 \mathbf{z} \\ \mathbf{A}_3 \mathbf{z} \end{bmatrix} = \begin{bmatrix} -\mathbf{A}_2 \mathbf{z} + \mathbf{A}_2 \mathbf{z} \\ \mathbf{A}_3 \mathbf{z} \end{bmatrix} = \begin{bmatrix} 0 \\ \mathbf{A}_3 \mathbf{z} \end{bmatrix}.$$

We can find a \mathbf{z} where $\mathbf{A}_3 \mathbf{z} = 0$.

Question 9

$$a(\mathbf{u} + \mathbf{v}) + b(\mathbf{u} + \mathbf{w}) + c(\mathbf{v} + \mathbf{w}) = \mathbf{0}.$$

Expanding, we get:

$$(a + b)\mathbf{u} + (a + c)\mathbf{v} + (b + c)\mathbf{w} = \mathbf{0}.$$

From this, we have:

$$a + b = 0, \quad a + c = 0, \quad b + c = 0.$$

Solving the equations:

$$a + b = 0 \implies a = -b,$$

$$a + c = 0 \implies a = -c,$$

$$b + c = 0 \implies c = -b.$$

Substituting $c = -b$ into $a = -c$, we get:

$$a = b.$$

Thus, we have:

$$a = b = c = 0.$$

Question 10

1. Non-emptiness: For \mathbf{W} , each vector \mathbf{W} is a subspace of \mathbf{V} .

$$\mathbf{0} \in \mathbf{W} \implies \forall \mathbf{v} \in \mathbf{W}, \mathbf{0} \in \mathcal{M}.$$

2. Closed under addition: If $\mathbf{u}, \mathbf{v} \in \mathcal{M}$, then $\mathbf{u} + \mathbf{v} \in \mathbf{W}$.

$$\forall \mathbf{u}, \mathbf{v} \in \mathbf{W}, \mathbf{u} + \mathbf{v} \in \mathcal{M}.$$

3. Closed under scalar multiplication: Let $\mathbf{u} \in \mathcal{M}$ and $c \in \mathbb{F}$ (where \mathbb{F} is the field over which \mathbf{V} is defined).

$$\forall \mathbf{u} \in \mathbf{W}, c\mathbf{u} \in \mathbf{W}.$$

Since \mathbf{W} is closed under scalar multiplication:

$$\forall \mathbf{u} \in \mathbf{W}, c\mathbf{u} \in \mathcal{M} \implies c\mathbf{u} \in \mathcal{M}.$$